Admitted to be removed

src/AbstractBigraphs.v
@@ -33,6 +33,16 @@ Import ListNotations.
 
 Module Bigraph.
 
+Fixpoint merge_list {A B : Type} (la : list A) (lb : list B) (acc : list (A + B)) : list (A + B) :=
+  match la with
+  | [] => acc ++ (map inr lb)
+  | ha :: ta => merge_list ta lb ((inl ha) :: acc)
+  end.
+  
+Definition merge {A B : Type} (la : list A) (lb : list B) : list (A + B) :=
+  merge_list la lb [].
+
+  
 Definition finite (A : Type) : Type := { l : list A | Listing l }.
 
 Definition acyclic (node site root : Type) (parent : node + site -> node + root) : Prop :=
@@ -52,14 +62,6 @@ Record bigraph (site: Type) (innername: Type) (root: Type) (outername: Type) (ki
     control : node -> kind * nat; (* k * nat *)
     parent : node + site -> node + root ; 
     link : innername + Port node kind control -> outername + edge; 
-    (* sd : EqDec site ;
-    sf : finite site ;
-    id_ : EqDec innername ;
-    if_ : finite innername ;
-    rd : EqDec root ;
-    rf : finite root ;
-    od : EqDec outername ;
-    of : finite outername ; *)
     nd : EqDec node ;
     nf : finite node ;
     ed : EqDec edge ;
@@ -190,161 +192,207 @@ Definition mk_new_link {s1 i1 r1 o1 k1 s2 i2 r2 o2 k2 : Type}
 
 
 
-Definition juxtaposition {s1 i1 r1 o1 k1 s2 i2 r2 o2 k2 : Type} 
-  (b1 : bigraph s1 i1 r1 o1 k1) (b2 : bigraph s2 i2 r2 o2 k2) 
-    : bigraph (s1+s2)%type (i1+i2)%type (r1+r2)%type (o1+o2)%type (k1+k2)%type :=
-  {|
-    node := (getNode b1) + (getNode b2) ;
-    edge := (getEdge b1) + (getEdge b2) ;
-    control := mk_new_control b1 b2 ;
-    parent := mk_new_parent b1 b2 ;
-    link := mk_new_link b1 b2 ;
-  |}.
-
+Definition getNd {s i r o k : Type} (bg : bigraph s i r o k) : 
+  EqDec (getNode bg) :=
+  @nd s i r o k bg.
+Definition mk_new_nd {s1 i1 r1 o1 k1 s2 i2 r2 o2 k2 : Type} 
+  (b1 : bigraph s1 i1 r1 o1 k1) (b2 : bigraph s2 i2 r2 o2 k2) :
+  EqDec ((getNode b1) + (getNode b2)).
+  Proof.  
+    (*destruct (getNd b1). EqDec. as [l1 H1]. 
+    destruct (getNd b2) as [l2 H2].*)
+    Admitted.
+Definition getNf {s i r o k : Type} (bg : bigraph s i r o k) : 
+  finite (getNode bg) :=
+  @nf s i r o k bg.
   
-  (* COMMENTS former juxtaposition function
-    let new_node : Type := (node b1 + node b2)%type in
-    (* let eqdec_newnode := fun a b =>
-      match a, b with
-      | inl a1, inl b1 => nd a1 b1
-      | inr a2, inr b2 => nd a2 b2
-      | _, _ => False
-      end in *)
-    let new_edge : Type := ((edge b1) + (edge b2))%type in
-    let new_kind : Type := (k1 + k2)%type in
-    (* let new_arity (k : new_kind) : nat := 
-      match k with
-      | inl k1 => arity b1 k1 
-      | inr k2 => arity b2 k2
-      end  
-    in *)
-    let new_control (n : new_node) : new_kind * nat := 
-      match n with
-      | inl n1 => (inl (fst (control n1)), snd (control n1))
-      | inr n2 => (inr (fst (control n2)), snd (control n2))
-      end 
-    in
-    let new_parent (p : new_node + (s1 + s2)) : new_node + (r1 + r2) :=
-      match p with
-      | inl node =>  match node with 
-                      |inl n1 => match parent (inl n1) with
-                                | inl n1' => inl (inl n1')
-                                | inr r1 => inr (inl r1)
-                                end
-                      |inr n2 => match parent (inl n2) with
-                                | inl n2' => inl (inr n2')
-                                | inr r2 => inr (inr r2)
-                                end
-                      end
-      | inr site => match site with 
-                    |inl s1 => match parent (inr s1) with
+Definition mk_new_nf {s i r o k : Type} 
+  (bg : bigraph s i r o k) (bg' : bigraph s i r o k) :
+  finite ((getNode bg) + (getNode bg')). 
+  Proof. 
+    destruct (getNf bg) as [l1 H1]. 
+    destruct (getNf bg') as [l2 H2].
+    unfold finite. 
+    (* exists (merge l1 l2). 
+    unfold merge. unfold merge_list.  *)
+    Admitted.
+Definition mk_new_nf' {s1 i1 r1 o1 k1 s2 i2 r2 o2 k2 : Type} 
+  (b1 : bigraph s1 i1 r1 o1 k1) (b2 : bigraph s2 i2 r2 o2 k2) :
+  finite ((getNode b1) + (getNode b2)). 
+  Proof. 
+    destruct (getNf b1) as [l1 H1]. 
+    destruct (getNf b2) as [l2 H2].
+    unfold finite. Admitted.  
+Definition mk_new_ed {s1 i1 r1 o1 k1 s2 i2 r2 o2 k2 : Type} 
+  (b1 : bigraph s1 i1 r1 o1 k1) (b2 : bigraph s2 i2 r2 o2 k2) :
+  EqDec ((getEdge b1) + (getEdge b2)). Admitted.
+Definition mk_new_ef {s1 i1 r1 o1 k1 s2 i2 r2 o2 k2 : Type} 
+  (b1 : bigraph s1 i1 r1 o1 k1) (b2 : bigraph s2 i2 r2 o2 k2) :
+  finite ((getEdge b1) + (getEdge b2)). Admitted.
+Definition mk_new_ap {s1 i1 r1 o1 k1 s2 i2 r2 o2 k2 : Type} 
+  (b1 : bigraph s1 i1 r1 o1 k1) (b2 : bigraph s2 i2 r2 o2 k2) :
+  acyclic ((getNode b1) + (getNode b2)) (s1 + s2) (r1 + r2) (mk_new_parent b1 b2). Admitted.
+
+  Definition juxtaposition {s1 i1 r1 o1 k1 s2 i2 r2 o2 k2 : Type} 
+(b1 : bigraph s1 i1 r1 o1 k1) (b2 : bigraph s2 i2 r2 o2 k2) 
+  : bigraph (s1+s2)%type (i1+i2)%type (r1+r2)%type (o1+o2)%type (k1+k2)%type :=
+{|
+  node := (getNode b1) + (getNode b2) ;
+  edge := (getEdge b1) + (getEdge b2) ;
+  control := mk_new_control b1 b2 ;
+  parent := mk_new_parent b1 b2 ;
+  link := mk_new_link b1 b2 ;
+  nd := mk_new_nd b1 b2 ;
+  nf := mk_new_nf' b1 b2 ;
+  ed := mk_new_ed b1 b2 ;
+  ef := mk_new_ef b1 b2 ;
+  ap := mk_new_ap b1 b2 ;
+|}.
+
+
+(* COMMENTS former juxtaposition function
+  let new_node : Type := (node b1 + node b2)%type in
+  (* let eqdec_newnode := fun a b =>
+    match a, b with
+    | inl a1, inl b1 => nd a1 b1
+    | inr a2, inr b2 => nd a2 b2
+    | _, _ => False
+    end in *)
+  let new_edge : Type := ((edge b1) + (edge b2))%type in
+  let new_kind : Type := (k1 + k2)%type in
+  (* let new_arity (k : new_kind) : nat := 
+    match k with
+    | inl k1 => arity b1 k1 
+    | inr k2 => arity b2 k2
+    end  
+  in *)
+  let new_control (n : new_node) : new_kind * nat := 
+    match n with
+    | inl n1 => (inl (fst (control n1)), snd (control n1))
+    | inr n2 => (inr (fst (control n2)), snd (control n2))
+    end 
+  in
+  let new_parent (p : new_node + (s1 + s2)) : new_node + (r1 + r2) :=
+    match p with
+    | inl node =>  match node with 
+                    |inl n1 => match parent (inl n1) with
                               | inl n1' => inl (inl n1')
                               | inr r1 => inr (inl r1)
                               end
-                    |inr s2 => match parent (inr s2) with
+                    |inr n2 => match parent (inl n2) with
                               | inl n2' => inl (inr n2')
                               | inr r2 => inr (inr r2)
                               end
-      end
-    end
-    in
-    (*let new_port : Type := 
-      ({x : node b1 * nat | snd x < snd (control (fst x))} + 
-      {x : node b2 * nat | snd x < snd (control (fst x))})%type
-    in*)
-    let new_link (i : (i1 + i2) + (Port new_control)): (o1 + o2) + new_edge := 
-      mk_new_link i
-    in
-    (* let new_link (i : (i1 + i2) + (Port new_control)): (o1 + o2) + new_edge := 
-      match i with
-      | inl innername => match innername with 
-                        |inl i1 =>  match link (inl i1) with
-                                    | inl o1 => inl (inl o1)
-                                    | inr e1 => inr (inl e1)
-                                    end
-                        |inr i2 =>  match link (inl i2) with
-                                    | inl o2 => inl (inr o2)
-                                    | inr e2 => inr (inr e2)
-                                    end
-                        end
-      | inr port => match fst (proj1_sig port) with
-                    | inl n1 => let port1 := Port 
-                    
-                                match @link s1 i1 r1 o1 k1 b1 (inr port) with
-                                | inl ot1 => inl (inl ot1)
-                                | inr ed1 => inr (inl ed1)
-                                end
-                    | inr n2 => match link (inr port) with 
-                                | inl o2 => inl (inr o2)
-                                | inr e2 => inr (inr e2)
-                                end
                     end
-      end 
-    in *)
-    (* let new_ap : acyclic new_parent := ap in *)
-    {|
-      node := new_node ;
-      edge := new_edge ;
-      control := new_control ;
-      parent := new_parent ;
-      link := new_link ;
-      (* sd := EqDec site ;
-      sf := Finite site ;
-      id_ := EqDec innername ;
-      if_ := Finite innername ;
-      rd := EqDec root ;
-      rf : Finite root ;
-      od : EqDec outername ;
-      of : Finite outername ;
-      nd : EqDec node ;
-      nf : Finite node ;
-      ed : EqDec edge ;
-      ef : Finite edge ; *)
-      (* ap := new_ap *)
-    |}.
-    (* Big new_parent new_link (s1+s2)%type (i1+i2) (r1+r2) (o1+o2) new_node new_edge new_control. 
+    | inr site => match site with 
+                  |inl s1 => match parent (inr s1) with
+                            | inl n1' => inl (inl n1')
+                            | inr r1 => inr (inl r1)
+                            end
+                  |inr s2 => match parent (inr s2) with
+                            | inl n2' => inl (inr n2')
+                            | inr r2 => inr (inr r2)
+                            end
+    end
+  end
+  in
+  (*let new_port : Type := 
+    ({x : node b1 * nat | snd x < snd (control (fst x))} + 
+    {x : node b2 * nat | snd x < snd (control (fst x))})%type
+  in*)
+  let new_link (i : (i1 + i2) + (Port new_control)): (o1 + o2) + new_edge := 
+    mk_new_link i
+  in
+  (* let new_link (i : (i1 + i2) + (Port new_control)): (o1 + o2) + new_edge := 
+    match i with
+    | inl innername => match innername with 
+                      |inl i1 =>  match link (inl i1) with
+                                  | inl o1 => inl (inl o1)
+                                  | inr e1 => inr (inl e1)
+                                  end
+                      |inr i2 =>  match link (inl i2) with
+                                  | inl o2 => inl (inr o2)
+                                  | inr e2 => inr (inr e2)
+                                  end
+                      end
+    | inr port => match fst (proj1_sig port) with
+                  | inl n1 => let port1 := Port 
+                  
+                              match @link s1 i1 r1 o1 k1 b1 (inr port) with
+                              | inl ot1 => inl (inl ot1)
+                              | inr ed1 => inr (inl ed1)
+                              end
+                  | inr n2 => match link (inr port) with 
+                              | inl o2 => inl (inr o2)
+                              | inr e2 => inr (inr e2)
+                              end
+                  end
+    end 
+  in *)
+  (* let new_ap : acyclic new_parent := ap in *)
+  {|
+    node := new_node ;
+    edge := new_edge ;
+    control := new_control ;
+    parent := new_parent ;
+    link := new_link ;
+    (* sd := EqDec site ;
+    sf := Finite site ;
+    id_ := EqDec innername ;
+    if_ := Finite innername ;
+    rd := EqDec root ;
+    rf : Finite root ;
+    od : EqDec outername ;
+    of : Finite outername ;
+    nd : EqDec node ;
+    nf : Finite node ;
+    ed : EqDec edge ;
+    ef : Finite edge ; *)
+    (* ap := new_ap *)
+  |}.
+  (* Big new_parent new_link (s1+s2)%type (i1+i2) (r1+r2) (o1+o2) new_node new_edge new_control. 
 
-    { node := new_node ;
-      edge := new_edge ;
-      control := new_control ;
-      parent := new_parent ;
-      link := new_link }.
+  { node := new_node ;
+    edge := new_edge ;
+    control := new_control ;
+    parent := new_parent ;
+    link := new_link }.
 
-    Big (node := new_node) (edge := new_edge) (control := new_control)
-        (parent := new_parent) (link := new_link) (sd := sum_dec (sd b1) (sd b2))
-        (sf := sum_finite (sf b1) (sf b2)) (id_ := sum_dec (id_ b1) (id_ b2))
-        (if_ := sum_finite (if_ b1) (if_ b2)) (rd := sum_dec (rd b1) (rd b2))
-        (rf := sum_finite (rf b1) (rf b2)) (od := sum_dec (od b1) (od b2))
-        (of := sum_finite (of b1) (of b2)) (nd := sum_dec (nd b1) (nd b2))
-        (nf := sum_finite (nf b1) (nf b2)) (ed := sum_dec (ed b1) (ed b2))
-        (ef := sum_finite (ef b1) (ef b2)). *) *)
+  Big (node := new_node) (edge := new_edge) (control := new_control)
+      (parent := new_parent) (link := new_link) (sd := sum_dec (sd b1) (sd b2))
+      (sf := sum_finite (sf b1) (sf b2)) (id_ := sum_dec (id_ b1) (id_ b2))
+      (if_ := sum_finite (if_ b1) (if_ b2)) (rd := sum_dec (rd b1) (rd b2))
+      (rf := sum_finite (rf b1) (rf b2)) (od := sum_dec (od b1) (od b2))
+      (of := sum_finite (of b1) (of b2)) (nd := sum_dec (nd b1) (nd b2))
+      (nf := sum_finite (nf b1) (nf b2)) (ed := sum_dec (ed b1) (ed b2))
+      (ef := sum_finite (ef b1) (ef b2)). *) *)
 
-  Definition mySite : Type := nat.
-  Definition myInnerName : Type := nat.
-  Definition myRoot : Type := nat.
-  Definition myOuterName : Type := nat.
-  Definition myKind : Type := nat.
-  Definition myNode : Type := {n:nat | n<3}.
-  Definition myEdge : Type := nat.
-  
-  Definition myControl : myNode -> nat * nat := fun _ => (10, 20).
-  Definition myParent : myNode + mySite -> myNode + myRoot := fun _ => inr 2.
-  Definition myLink : myInnerName + {x : myNode * nat | snd x < snd (myControl (fst x))} -> 
-    myOuterName + myEdge := fun _ => inr 1.
+Definition mySite : Type := nat.
+Definition myInnerName : Type := nat.
+Definition myRoot : Type := nat.
+Definition myOuterName : Type := nat.
+Definition myKind : Type := nat.
+Definition myNode : Type := {n:nat | n<3}.
+Definition myEdge : Type := nat.
 
-
-  Definition Full (l:list myNode) :=
-  forall n:myNode, In n l.
+Definition myControl : myNode -> nat * nat := fun _ => (10, 20).
+Definition myParent : myNode + mySite -> myNode + myRoot := fun _ => inr 2.
+Definition myLink : myInnerName + {x : myNode * nat | snd x < snd (myControl (fst x))} -> 
+  myOuterName + myEdge := fun _ => inr 1.
 
 
-  Definition node0 : myNode.
-  Proof. unfold myNode. exists 0. auto. Qed.
+Definition Full (l:list myNode) :=
+forall n:myNode, In n l.
 
-  Definition node1 : myNode.
-  Proof. unfold myNode. exists 1. auto. Qed.
 
-  Definition node2 : myNode.
-  Proof. unfold myNode. exists 2. auto. Qed.
+Definition node0 : myNode.
+Proof. unfold myNode. exists 0. auto. Qed.
+
+Definition node1 : myNode.
+Proof. unfold myNode. exists 1. auto. Qed.
+
+Definition node2 : myNode.
+Proof. unfold myNode. exists 2. auto. Qed.
 
 
 
